Updated theory Bmethod with recent changes. Fixed errors in text (Simulation.thy).

Bmethod.thy
@@ -33,18 +33,29 @@ proof-
   then show ?thesis by (simp only:sound_B_machine_def)
 qed
 
-section {* B refinement: two components glued by a relation between states *}
+section {* B refinement *}
+
+text {* A B refinement is composed of an \emph{abstract} component and a \emph{concrete}
+component related by an \emph{invariant}. The invariant is a binary relation from the states 
+of the abstract component to the states of the concrete one. *}
 
 record ('st, 'ev) B_refinement =
-  abstract :: "('st, 'ev) LTS"
-  concrete :: "('st, 'ev) LTS"
-  invariant :: "'st \<times> 'st \<Rightarrow> bool" (* relates Abstract to Concrete - see wd_B_refinement_glue *)
+  abstract :: "('st, 'ev) LTS" -- "the abstract component"
+  concrete :: "('st, 'ev) LTS"  -- "the concrete component "
+  invariant :: "'st \<times> 'st \<Rightarrow> bool" -- "relates the abstract to the concrete component"
   
-definition sound_B_refinement :: "('st, 'ev) B_refinement \<Rightarrow> bool" where
-"sound_B_refinement r \<equiv> simulation (Collect (invariant r)) (concrete r) (abstract r)"
+text {* A refinement is considered \emph{sound} if the invariant establishes a simulation
+from the concrete component by the abstract component: every execution of the former corresponds
+to some execution of the latter. Isabelle's operator @{text "Collect"}, applied to a relation,
+returns its characteristic predicate. *}
 
-lemma "sound_B_refinement r \<Longrightarrow> simulates (abstract r) (concrete r)"
-unfolding sound_B_refinement_def simulates_def by auto
+definition sound_B_refinement :: "('st, 'ev) B_refinement \<Rightarrow> bool" where
+  "sound_B_refinement r \<equiv> simulation (Collect (invariant r)) (concrete r) (abstract r)"
+
+text {* Thus, in a refinement, the abstract component simulates its concrete counterpart: *}
+
+lemma refinement_sim: "\<lbrakk> sound_B_refinement r \<rbrakk> \<Longrightarrow> (abstract r) \<sim> (concrete r)"
+  unfolding sound_B_refinement_def simulates_def by auto
 
 text {* A special refinement is one that does not change anything, namely the
 identity refinement. It is defined as a function that takes a machine and
@@ -53,15 +64,14 @@ returns the identity refinement. *}
 definition refinement_id :: "('st, 'ev) LTS \<Rightarrow> ('st, 'ev) B_refinement" where
 "refinement_id m \<equiv> \<lparr> abstract = m, concrete = m, invariant = (\<lambda> p . fst p = snd p) \<rparr>"
 
-text {* We have that the identity refinement is sound. *}
+text {* The identity refinement is sound: *}
 
 lemma "sound_B_refinement(refinement_id m)"
-unfolding sound_B_refinement_def refinement_id_def simulation_def simulation_init_def simulation_step_def 
+unfolding refinement_id_def sound_B_refinement_def simulation_def sim_lts_init_def sim_lts_trans_def sim_transition_def
 by auto
 
-text {* Next, we definement composition of refinements. This is only defined if the
-composed refinements have matching set of states, otherwise it is left
-undefined. *}
+text {* Next, we definement composition of refinements. This is a partial operation as it is only 
+meaningful when the composed refinements have matching set of states. *}
 
 definition refinement_compose :: "('st, 'ev) B_refinement \<Rightarrow> ('st, 'ev) B_refinement \<Rightarrow> ('st, 'ev) B_refinement option" where
 "refinement_compose r1 r2 \<equiv> 
@@ -70,11 +80,22 @@ definition refinement_compose :: "('st, 'ev) B_refinement \<Rightarrow> ('st, 'e
          invariant = \<lambda> p . p \<in> Collect (invariant r2) O Collect (invariant r1) \<rparr>
   else None)"
 
+text {* The following lemma states that the composition of two refinements @{text "r1"} and
+@{text "r2"} is defined whenever the concrete component of @{text "r1"} and the abstract
+component of @{text "r2"} are equal. The abstract (resp. concrete) component of the result
+are the abstract (resp. concrete) component of @{text "r1"} (resp. @{text "r2"}), and the
+invariant is obtained by relational composition of the invariants of @{text "r1"} and @{text "r2"}.*}
+
 lemma refinement_compose_matching:
-  "concrete r1 = abstract r2 \<Longrightarrow>
-   refinement_compose r1 r2 = Some \<lparr> abstract = abstract r1, concrete = concrete r2, 
-         invariant = \<lambda> p . p \<in> Collect (invariant r2) O Collect (invariant r1) \<rparr>"
+  "\<lbrakk> concrete r1 = abstract r2 \<rbrakk> \<Longrightarrow>
+   refinement_compose r1 r2 = 
+     Some \<lparr> abstract = abstract r1,
+            concrete = concrete r2, 
+            invariant = \<lambda> p . p \<in> Collect (invariant r2) O Collect (invariant r1) \<rparr>"
 unfolding refinement_compose_def by auto
+
+text {* The composition of two sound refinements, when it is defined, is sound. This is 
+the object of the following lemma @{text "refinement_compose_soundness"}: *}
 
 lemma refinement_compose_soundness:
   assumes 
@@ -102,8 +123,8 @@ next
       unfolding simulation_def sound_B_refinement_def rs2_def by auto
     with sound_r1 and glue have rs1: "simulation rs1 (abstract r2) (abstract r1)"
       unfolding simulation_def sound_B_refinement_def rs1_def by auto
-    with rs2 have "simulation (rs2 O rs1) (concrete r2) (abstract r1)" 
-      by (rule Simulation.simulation_transitivity[of "rs2" "concrete r2" "abstract r2" "rs1" "abstract r1"])
+    with rs2 have "simulation (rs2 O rs1) (concrete r2) (abstract r1)"  
+      by (metis simulation_closed)
     with value_r show "simulation (Collect (invariant r)) (concrete r) (abstract r)"
       unfolding rv_def rs1_def rs2_def by simp
   qed
@@ -163,43 +184,67 @@ qed
 text {* Last, refinement composition is associative. The expression of this
 property is not as straightforward as we could expect due to the partialness
 of composition. *}
+
 lemma refinement_compose_associative:
-  assumes "sound_B_refinement r1 \<and> sound_B_refinement r2 \<and> sound_B_refinement r3"
-      and "concrete r1 = abstract r2" 
-      and "concrete r2 = abstract r3"
-  shows "\<exists> r12 r23 . Some r12 = refinement_compose r1 r2 \<and> 
+  "\<lbrakk> sound_B_refinement r1; sound_B_refinement r2; sound_B_refinement r3;
+     concrete r1 = abstract r2; concrete r2 = abstract r3 \<rbrakk> \<Longrightarrow>
+  \<exists> r12 r23 . Some r12 = refinement_compose r1 r2 \<and> 
          Some r23 = refinement_compose r2 r3 \<and>
          refinement_compose r12 r3 = refinement_compose r1 r23"
 proof(simp add:sound_B_refinement_def refinement_compose_def, auto)
-  from assms(2) show "concrete r1 = abstract r2" by simp
-next
-  from assms(3) show "concrete r2 = abstract r3" by simp
 qed
 
 section {* B development *}
 
+text {* A B development is a specification and the development of an implementation of that
+specification by stepwise refinements. We first provide a formalization of design, as a list
+of refinements: *}
+
 type_synonym ('st, 'ev) B_design = "('st, 'ev) B_refinement list"
+
+text {* We specify a predicate @{text "sound_B_design"}, responsible for identifying sound 
+developments: each refinement is sound, and the chain of refinements is continuous, i.e. the
+concrete component of a refinement is the abstract component of the next refinement: *}
 
 inductive sound_B_design :: "('st, 'ev) B_design \<Rightarrow> bool" where
   base: "sound_B_design []" |
-  step: "\<lbrakk> sound_B_refinement x; xs \<noteq> [] \<longrightarrow> concrete x = abstract (hd xs) \<and> sound_B_design xs \<rbrakk> \<Longrightarrow> sound_B_design (x # xs)"
-   
+  step: "\<lbrakk> sound_B_refinement x; xs \<noteq> []; concrete x = abstract (hd xs); sound_B_design xs \<rbrakk> \<Longrightarrow> 
+           sound_B_design (x # xs)"
+
+text {* In such a design, by transitivity of the simulates relation, the abstract component of the 
+first refinement simulates the concrete component of the last refinement: *}
+
 lemma 
-"sound_B_design dev \<Longrightarrow> dev \<noteq> [] \<Longrightarrow> simulates (abstract(hd dev)) (concrete (last dev))"
-unfolding sound_B_design_def sound_B_refinement_def
-sorry
+  design_sim: "\<lbrakk> sound_B_design dev; dev \<noteq> [] \<rbrakk>  \<Longrightarrow> (abstract(hd dev)) \<sim> (concrete (last dev))"
+proof(induct rule:sound_B_design.induct, simp, simp)
+  fix x xs
+  assume "sound_B_refinement x" "concrete x = abstract (hd xs)"
+         "abstract (hd xs) \<sim> concrete (last xs)"
+  from `sound_B_refinement x` have "abstract x \<sim> concrete x" by (rule refinement_sim)
+  with `concrete x = abstract (hd xs)` `abstract (hd xs) \<sim> concrete (last xs)`
+  show "abstract x \<sim> concrete (last xs)" by (metis simulates_transitivity)
+qed
+
+text {* Eventually, we give a formalization of a B development as a pair formed by a specification,
+namely a B machine, and a design: *}
 
 record ('st, 'ev) B_development =
   spec :: "('st, 'ev) B_machine"
   design :: "('st, 'ev) B_design"
 
+text {* Then a B development is sound when the machine and the design are sound. Moreover, the
+design must have the specification machine as initial abstract component: *}
+
 definition sound_B_development :: "('st, 'ev) B_development \<Rightarrow> bool" where
   "sound_B_development dev \<equiv> 
     sound_B_machine (spec dev) \<and> sound_B_design (design dev) \<and>
-    (design dev \<noteq> [] \<longrightarrow> (B_machine.lts (spec dev)) = (abstract (hd (design dev))))"
+    (design dev \<noteq> [] \<longrightarrow> (lts (spec dev)) = (abstract (hd (design dev))))"
 
-definition B_implementation :: "('st, 'ev) B_development \<Rightarrow> ('st, 'ev) LTS" where
-  "B_implementation dev \<equiv> 
-    (if design dev = [] then B_machine.lts (spec dev) else concrete (last (design dev)))"
+text {* The following theorem states that, in a sound B development, the initial specification
+  simulates the concrete component of the final refinement of the design: *}
+
+theorem development_sim: 
+  "\<lbrakk> sound_B_development d ; design d \<noteq> [] \<rbrakk> \<Longrightarrow> lts (spec d) \<sim> concrete (last (design d))"
+  by(metis design_sim sound_B_development_def)
 
 end
